Prove eq_dec dvalue

src/coq/DecidableEquality.v
@@ -394,7 +394,7 @@ Proof.
          IH_Select.
 
   refine
-    (fix prove_dv (v : Ollvm_ast.value ) :=
+    (fix prove_v (v : Ollvm_ast.value ) :=
        match v with
          | VALUE_Ident id => _
          | VALUE_Integer n => _
@@ -411,7 +411,7 @@ Proof.
              match l with
              | [] => IH_Struct_Base
              | (t, v) :: rest =>
-               IH_Struct_Ind t v rest (prove_dv v) (prove_l rest)
+               IH_Struct_Ind t v rest (prove_v v) (prove_l rest)
              end
            in prove_l l 
          | VALUE_Packed_struct l =>
@@ -420,7 +420,7 @@ Proof.
              match l with
              | [] => IH_Packed_struct_Base
              | (t, v) :: rest =>
-               IH_Packed_struct_Ind t v rest (prove_dv v) (prove_l rest)
+               IH_Packed_struct_Ind t v rest (prove_v v) (prove_l rest)
              end
            in prove_l l 
          | VALUE_Array l =>
@@ -429,7 +429,7 @@ Proof.
              match l with
              | [] => IH_Array_Base
              | (t, v) :: rest =>
-               IH_Array_Ind t v rest (prove_dv v) (prove_l rest)
+               IH_Array_Ind t v rest (prove_v v) (prove_l rest)
              end
            in prove_l l 
 
@@ -439,50 +439,50 @@ Proof.
              match l with
              | [] => IH_Vector_Base
              | (t, v) :: rest =>
-               IH_Vector_Ind t v rest (prove_dv v) (prove_l rest)
+               IH_Vector_Ind t v rest (prove_v v) (prove_l rest)
              end
            in prove_l l            
 
          | OP_IBinop op t v1 v2 =>
-           IH_IBinop op t v1 v2 (prove_dv v1) (prove_dv v2) 
+           IH_IBinop op t v1 v2 (prove_v v1) (prove_v v2) 
          | OP_ICmp op t v1 v2 => 
-           IH_ICmp op t v1 v2 (prove_dv v1) (prove_dv v2) 
+           IH_ICmp op t v1 v2 (prove_v v1) (prove_v v2) 
          | OP_FBinop op fm t v1 v2 =>
-           IH_FBinop op fm t v1 v2 (prove_dv v1) (prove_dv v2) 
+           IH_FBinop op fm t v1 v2 (prove_v v1) (prove_v v2) 
          | OP_FCmp op t v1 v2 =>
-           IH_FCmp op t v1 v2 (prove_dv v1) (prove_dv v2) 
+           IH_FCmp op t v1 v2 (prove_v v1) (prove_v v2) 
          | OP_Conversion conv t_from v t_to =>
-           IH_Conversion conv t_from v t_to (prove_dv v)
+           IH_Conversion conv t_from v t_to (prove_v v)
            
          | OP_GetElementPtr t (ptr_t, ptr_v) l =>
            let fix prove_l (l : list (Ollvm_ast.typ * Ollvm_ast.value)) :=
                match l with
                | [] =>
-                 IH_GetElementPtr_Base t ptr_t ptr_v (prove_dv ptr_v)
+                 IH_GetElementPtr_Base t ptr_t ptr_v (prove_v ptr_v)
                | (idx_t, idx_v) :: rest =>
                  IH_GetElementPtr_Ind t ptr_t ptr_v idx_t idx_v rest
-                                      (prove_dv ptr_v) (prove_dv idx_v)
+                                      (prove_v ptr_v) (prove_v idx_v)
                                       (prove_l rest)
                end
            in prove_l l
            
          | OP_ExtractElement (vec_t, vec_v) (idx_t, idx_v) =>
            IH_ExtractElement vec_t vec_v idx_t idx_v
-                             (prove_dv vec_v) (prove_dv idx_v)
+                             (prove_v vec_v) (prove_v idx_v)
          | OP_InsertElement (vec_t, vec_v) (elt_t, elt_v) (idx_t, idx_v) =>
            IH_InsertElement vec_t vec_v elt_t elt_v idx_t idx_v
-                            (prove_dv vec_v) (prove_dv elt_v) (prove_dv idx_v)
+                            (prove_v vec_v) (prove_v elt_v) (prove_v idx_v)
          | OP_ShuffleVector (vec1_t, vec1_v) (vec2_t, vec2_v) (idxmask_t, idxmask_v) => 
            IH_ShuffleVector vec1_t vec1_v vec2_t vec2_v idxmask_t idxmask_v
-                            (prove_dv vec1_v) (prove_dv vec2_v) (prove_dv idxmask_v)
+                            (prove_v vec1_v) (prove_v vec2_v) (prove_v idxmask_v)
          | OP_ExtractValue (vec_t, vec_v) idxs =>
-           IH_ExtractValue vec_t vec_v idxs (prove_dv vec_v) 
+           IH_ExtractValue vec_t vec_v idxs (prove_v vec_v) 
          | OP_InsertValue (vec_t, vec_v) (elt_t, elt_v) idxs =>
            IH_InsertValue vec_t vec_v elt_t elt_v idxs
-                          (prove_dv vec_v) (prove_dv elt_v)
+                          (prove_v vec_v) (prove_v elt_v)
          | OP_Select (cnd_t, cnd_v) (v1_t, v1_v) (v2_t, v2_v) =>
            IH_Select cnd_t cnd_v v1_t v1_v v2_t v2_v
-                     (prove_dv cnd_v) (prove_dv v1_v) (prove_dv v2_v)
+                     (prove_v cnd_v) (prove_v v1_v) (prove_v v2_v)
          end
     ); auto.
 Defined.
@@ -815,210 +815,85 @@ Proof.
     { intros H; inversion H; apply cnd_t_neq; subst; auto. }
 Defined.
 
-(*
-Definition expr_dvalue_ind: forall (P : dvalue -> Set),
-    (forall id : ident, P (DV (VALUE_Ident id))) ->
-    (forall x : int, P (DV (VALUE_Integer x))) ->
-    (forall f : float, P (DV (VALUE_Float f))) ->
-    (forall h : String.string, P (DV (VALUE_Hex h))) ->    
-    (forall b : bool, P (DV (VALUE_Bool b))) ->
-    (P (DV VALUE_Null)) ->
-    (P (DV (VALUE_Zero_initializer))) ->
-    (forall s : String.string, P (DV (VALUE_Cstring s))) ->
-    (P (DV VALUE_None)) ->
-    (P (DV VALUE_Undef)) ->
-    (P (DV (VALUE_Struct []))) ->
-    (forall t v fields,
-        P v ->
-        P (DV (VALUE_Struct fields)) ->
-        P (DV (VALUE_Struct ((t, v) :: fields)))) ->
-    (P (DV (VALUE_Packed_struct []))) ->
-    (forall t v fields,
-        P v ->
-        P (DV (VALUE_Packed_struct fields)) ->
-        P (DV (VALUE_Packed_struct ((t, v) :: fields)))) ->
-    (P (DV (VALUE_Array []))) ->
-    (forall t v arr,
-        P v ->
-        P (DV (VALUE_Array arr)) ->
-        P (DV (VALUE_Array ((t, v) :: arr)))) ->
-    (P (DV (VALUE_Vector []))) ->
-    (forall t v vec,
-        P v ->
-        P (DV (VALUE_Vector vec)) ->
-        P (DV (VALUE_Vector ((t, v) :: vec)))) ->
-    (forall iop t v1 v2,
-        P v1 -> P v2 ->
-        P (DV (OP_IBinop iop t v1 v2))) ->
-    (forall cmp t v1 v2,
-        P v1 -> P v2 ->
-        P (DV (OP_ICmp cmp t v1 v2))) ->
-    (forall fop fm t v1 v2,
-        P v1 -> P v2 ->
-        P (DV (OP_FBinop fop fm t v1 v2))) ->
-    (forall cmp t v1 v2,
-        P v1 -> P v2 ->
-        P (DV (OP_FCmp cmp t v1 v2))) ->
-    (forall conv t_from v t_to,
-        P v -> P (DV (OP_Conversion conv t_from v t_to))) ->
-    (forall t ptr_t ptr_v,
-        P (ptr_v) ->
-        P (DV (OP_GetElementPtr t (ptr_t, ptr_v) []))) ->
-    (forall t ptr_t ptr_v idx_t idx_v indices,
-        P (ptr_v) ->
-        P (idx_v) ->
-        P (DV (OP_GetElementPtr t (ptr_t, ptr_v) indices)) ->
-        P (DV (OP_GetElementPtr t (ptr_t, ptr_v) ((idx_t, idx_v) :: indices)))) ->
-    (forall vec_t vec_v idx_t idx_v,
-        P vec_v -> P idx_v -> P (DV (OP_ExtractElement (vec_t, vec_v) (idx_t, idx_v)))) ->
-    (forall vec_t vec_v elt_t elt_v idx_t idx_v,
-        P vec_v -> P elt_v -> P idx_v ->
-        P (DV (OP_InsertElement (vec_t, vec_v) (elt_t, elt_v) (idx_t, idx_v)))) ->
-    (forall vec1_t vec1_v vec2_t vec2_v idxmask_t idxmask_v,
-        P vec1_v -> P vec2_v -> P (idxmask_v) ->
-        P (DV (OP_ShuffleVector (vec1_t, vec1_v) (vec2_t, vec2_v) (idxmask_t, idxmask_v)))) ->
-    (forall vec_t vec_v idxs,
-        P vec_v -> P (DV (OP_ExtractValue (vec_t, vec_v) idxs))) ->
-    (forall vec_t vec_v elt_t elt_v idxs,
-        P vec_v -> P elt_v ->
-        P (DV (OP_InsertValue (vec_t, vec_v) (elt_t, elt_v) idxs))) ->
-    (forall cnd_t cnd_v v1_t v1_v v2_t v2_v,
-        P cnd_v -> P v1_v -> P v2_v ->
-        P (DV (OP_Select (cnd_t, cnd_v) (v1_t, v1_v) (v2_t, v2_v)))) ->
-
-    (forall p : instr_id, P (DVALUE_CodePointer p)) ->
-    (forall a : A.addr, P (DVALUE_Addr a)) ->
-    (forall x : Int1.int, P (DVALUE_I1 x)) ->
-    (forall x : Int32.int, P (DVALUE_I32 x)) ->
-    (forall x : Int64.int, P (DVALUE_I64 x)) ->
-    (P DVALUE_Poison) ->
-    (forall v : dvalue, P v).
-Proof.
-  intros P H_Ident H_Integer H_Float H_Hex H_Bool H_Null
-         H_Zero_initializer H_Cstring H_None H_Undef.
-  intros IH_Struct_Base IH_Struct_Ind
-         IH_Packed_struct_Base IH_Packed_struct_Ind
-         IH_Array_Base IH_Array_Ind
-         IH_Vector_Base IH_Vector_Ind
-         IH_IBinop IH_ICmp IH_FBinop IH_FCmp
-         IH_Conversion
-         IH_GetElementPtr_Base IH_GetElementPtr_Ind
-         IH_ExtractElement IH_InsertElement
-         IH_ShuffleVector IH_ExtractValue IH_InsertValue
-         IH_Select
-         H_CodePointer H_Addr H_I1 H_I32 H_I64 H_Poison.
-
-  refine
-    (fix prove_dv (v : dvalue) :=
-       match v with
-       | DV e =>
-         match e with
-         | VALUE_Ident id => _
-         | VALUE_Integer n => _
-         | VALUE_Float f => _
-         | VALUE_Hex h => _                             
-         | VALUE_Bool b => _
-         | VALUE_Null => _
-         | VALUE_Zero_initializer => _
-         | VALUE_Cstring s => _
-         | VALUE_None => _
-         | VALUE_Undef => _
-         | VALUE_Struct l =>
-           let
-             fix prove_l (l : list (Ollvm_ast.typ * dvalue)) :=
+Definition dvalue_ind':=
+  fun (P : dvalue -> Set) (f : forall p : instr_id, P (DVALUE_CodePointer p))
+    (f0 : forall a : A.addr, P (DVALUE_Addr a))
+    (f1 : forall x : int1, P (DVALUE_I1 x))
+    (f2 : forall x : int32, P (DVALUE_I32 x))
+    (f3 : forall x : int64, P (DVALUE_I64 x))
+    (f4 : forall x : ll_double, P (DVALUE_Double x))
+    (f5 : forall x : ll_float, P (DVALUE_Float x))
+    (f6 : forall (t : Ollvm_ast.typ) (v : option Ollvm_ast.value),
+          P (DVALUE_Undef t v)) (f7 : P DVALUE_Poison) 
+    (f8 : P DVALUE_None)
+    (IH_Struct_Base: P(DVALUE_Struct []))
+    (IH_Struct_Ind : forall t v fields, 
+          P v ->
+          P (DVALUE_Struct fields) ->
+          P (DVALUE_Struct ((t,v)::fields)))
+    (IH_Packed_Struct_Base: P(DVALUE_Packed_struct []))
+    (IH_Packed_Struct_Ind : forall t v fields,
+          P v ->
+          P (DVALUE_Packed_struct fields) ->
+          P (DVALUE_Packed_struct ((t,v) :: fields)))
+    (IH_Array_Base: P(DVALUE_Array []))
+    (IH_Array_Ind : forall t v elts , 
+          P v ->
+          P (DVALUE_Array elts) ->
+          P (DVALUE_Array ((t, v) :: elts)))
+    (IH_Vector_Base: P(DVALUE_Vector []))
+    (IH_Vector_Ind : forall t v elts, 
+          P v ->
+          P (DVALUE_Vector elts) ->
+          P (DVALUE_Vector ((t,v) :: elts)))
+     =>
+    fix prove_dv (d : dvalue) := match d as d0 return (P d0) with
+      | DVALUE_CodePointer x => f x
+      | DVALUE_Addr x => f0 x
+      | DVALUE_I1 x => f1 x
+      | DVALUE_I32 x => f2 x
+      | DVALUE_I64 x => f3 x
+      | DVALUE_Double x => f4 x
+      | DVALUE_Float x => f5 x
+      | DVALUE_Undef x x0 => f6 x x0
+      | DVALUE_Poison => f7
+      | DVALUE_None => f8
+      | DVALUE_Struct x =>
+        (fix prove_l (l : list (Ollvm_ast.typ * dvalue)) :=
              match l with
              | [] => IH_Struct_Base
              | (t, v) :: rest =>
                IH_Struct_Ind t v rest (prove_dv v) (prove_l rest)
-             end
-           in prove_l l 
-         | VALUE_Packed_struct l =>
-           let
-             fix prove_l (l : list (Ollvm_ast.typ * dvalue)) :=
+             end) x
+      | DVALUE_Packed_struct x =>         
+        (fix prove_l (l : list (Ollvm_ast.typ * dvalue)) :=
              match l with
-             | [] => IH_Packed_struct_Base
+             | [] => IH_Packed_Struct_Base
              | (t, v) :: rest =>
-               IH_Packed_struct_Ind t v rest (prove_dv v) (prove_l rest)
-             end
-           in prove_l l 
-         | VALUE_Array l =>
-           let
-             fix prove_l (l : list (Ollvm_ast.typ * dvalue)) :=
+               IH_Packed_Struct_Ind t v rest (prove_dv v) (prove_l rest)
+             end) x
+      | DVALUE_Array x =>          
+        (fix prove_l (l : list (Ollvm_ast.typ * dvalue)) :=
              match l with
              | [] => IH_Array_Base
              | (t, v) :: rest =>
                IH_Array_Ind t v rest (prove_dv v) (prove_l rest)
-             end
-           in prove_l l 
-
-         | VALUE_Vector l =>
-           let
-             fix prove_l (l : list (Ollvm_ast.typ * dvalue)) :=
+             end) x
+      | DVALUE_Vector x =>          
+        (fix prove_l (l : list (Ollvm_ast.typ * dvalue)) :=
              match l with
              | [] => IH_Vector_Base
              | (t, v) :: rest =>
                IH_Vector_Ind t v rest (prove_dv v) (prove_l rest)
-             end
-           in prove_l l            
-
-         | OP_IBinop op t v1 v2 =>
-           IH_IBinop op t v1 v2 (prove_dv v1) (prove_dv v2) 
-         | OP_ICmp op t v1 v2 => 
-           IH_ICmp op t v1 v2 (prove_dv v1) (prove_dv v2) 
-         | OP_FBinop op fm t v1 v2 =>
-           IH_FBinop op fm t v1 v2 (prove_dv v1) (prove_dv v2) 
-         | OP_FCmp op t v1 v2 =>
-           IH_FCmp op t v1 v2 (prove_dv v1) (prove_dv v2) 
-         | OP_Conversion conv t_from v t_to =>
-           IH_Conversion conv t_from v t_to (prove_dv v)
-           
-         | OP_GetElementPtr t (ptr_t, ptr_v) l =>
-           let fix prove_l (l : list (Ollvm_ast.typ * dvalue)) :=
-               match l with
-               | [] =>
-                 IH_GetElementPtr_Base t ptr_t ptr_v (prove_dv ptr_v)
-               | (idx_t, idx_v) :: rest =>
-                 IH_GetElementPtr_Ind t ptr_t ptr_v idx_t idx_v rest
-                                      (prove_dv ptr_v) (prove_dv idx_v)
-                                      (prove_l rest)
-               end
-           in prove_l l
-           
-         | OP_ExtractElement (vec_t, vec_v) (idx_t, idx_v) =>
-           IH_ExtractElement vec_t vec_v idx_t idx_v
-                             (prove_dv vec_v) (prove_dv idx_v)
-         | OP_InsertElement (vec_t, vec_v) (elt_t, elt_v) (idx_t, idx_v) =>
-           IH_InsertElement vec_t vec_v elt_t elt_v idx_t idx_v
-                            (prove_dv vec_v) (prove_dv elt_v) (prove_dv idx_v)
-         | OP_ShuffleVector (vec1_t, vec1_v) (vec2_t, vec2_v) (idxmask_t, idxmask_v) => 
-           IH_ShuffleVector vec1_t vec1_v vec2_t vec2_v idxmask_t idxmask_v
-                            (prove_dv vec1_v) (prove_dv vec2_v) (prove_dv idxmask_v)
-         | OP_ExtractValue (vec_t, vec_v) idxs =>
-           IH_ExtractValue vec_t vec_v idxs (prove_dv vec_v) 
-         | OP_InsertValue (vec_t, vec_v) (elt_t, elt_v) idxs =>
-           IH_InsertValue vec_t vec_v elt_t elt_v idxs
-                          (prove_dv vec_v) (prove_dv elt_v)
-         | OP_Select (cnd_t, cnd_v) (v1_t, v1_v) (v2_t, v2_v) =>
-           IH_Select cnd_t cnd_v v1_t v1_v v2_t v2_v
-                     (prove_dv cnd_v) (prove_dv v1_v) (prove_dv v2_v)
-         end
-         
-       | DVALUE_CodePointer p => _
-       | DVALUE_Addr a => _
-       | DVALUE_I1 x => _
-       | DVALUE_I32 x => _
-       | DVALUE_I64 x => _
-       | DVALUE_Poison => _
-       end
-    ); auto.
-Defined.  
+             end) x
+    end.
 
 Instance eq_dec_lldouble : eq_dec ll_double := Floats.Float.eq_dec.
 Instance eq_dec_llfloat : eq_dec ll_float := Floats.Float32.eq_dec.
 
 Instance eq_dvalue : eq_dec dvalue.
 Proof.
-  induction x; destruct y; 
+  induction x using dvalue_ind'; destruct y; 
     try (right; intro H; inversion H; tauto);
     try (lift_decide_eq);
     try destruct e; unfold Decidable;
@@ -1026,7 +901,7 @@ Proof.
       try solve [left; auto];
       try solve [lift_decide_eq].
 
-  (* DV (VALUE_Struct ...) *)
+  (* DVALUE_Struct ... *)
   - destruct fields; auto.
   - refine
       (match fields0 with
@@ -1036,8 +911,8 @@ Proof.
          | left t_eq =>
            match decide (x = v') with
            | left value_eq =>
-             match decide (DV (VALUE_Struct fields) =
-                           DV (VALUE_Struct fields')) with
+             match decide ((DVALUE_Struct fields) =
+                           (DVALUE_Struct fields')) with
              | left fields_eq => left _
              | right fields_neq => right _
              end
@@ -1052,7 +927,7 @@ Proof.
     { intros H; inversion H; apply value_neq; subst; auto. }
     { intros H; inversion H; apply t_neq; subst; auto. }
 
-    (* DV (VALUE_Packed_struct ...) *)
+    (* DVALUE_Packed_struct ... *)
   - destruct fields; auto.
   - refine
       (match fields0 with
@@ -1062,8 +937,8 @@ Proof.
          | left t_eq =>
            match decide (x = v') with
            | left value_eq =>
-             match decide (DV (VALUE_Packed_struct fields) =
-                           DV (VALUE_Packed_struct fields')) with
+             match decide (DVALUE_Packed_struct fields =
+                           DVALUE_Packed_struct fields') with
              | left fields_eq => left _
              | right fields_neq => right _
              end
@@ -1078,15 +953,15 @@ Proof.
     { intros H; inversion H; apply value_neq; subst; auto. }
     { intros H; inversion H; apply t_neq; subst; auto. }
 
-    (* DV (VALUE_Array ...) *)
+    (* DVALUE_Array ... *)
   - destruct elts; auto.
-  - destruct elts as [| (t', x') arr']; auto.
+  - destruct elts0 as [| (t', x') elts']; auto.
     refine
       (match (decide (t = t')) with
        | left t_eq =>
          match (decide (x = x')) with
          | left value_eq =>
-           match decide (DV (VALUE_Array arr) = DV (VALUE_Array arr')) with
+           match decide (DVALUE_Array elts = DVALUE_Array elts') with
            | left rest_eq => left _
            | right rest_neq => right _
            end
@@ -1101,13 +976,13 @@ Proof.
 
     (* DV (VALUE_Vector *)
   - destruct elts; auto.
-  - destruct elts as [| (t', x') vec']; auto.
+  - destruct elts0 as [| (t', x') elts']; auto.
     refine
       (match (decide (t = t')) with
        | left t_eq =>
          match (decide (x = x')) with
          | left value_eq =>
-           match decide (DV (VALUE_Vector vec) = DV (VALUE_Vector vec')) with
+           match decide (DVALUE_Vector elts = DVALUE_Vector elts') with
            | left rest_eq => left _
            | right rest_neq => right _
            end
@@ -1120,13 +995,6 @@ Proof.
     { intros H; inversion H; apply value_neq; subst; auto. }
     { intros H; inversion H; apply t_neq; subst; auto. }
 Defined.
-*)
-
-(*
-Instance eq_dec_static_value : eq_dec Ollvm_ast.value.
-Proof.
-  unfold Decidable.
-  induction x using value_ind'.
 
 Instance eq_dec_instr : eq_dec instr.
 Proof.
@@ -1158,7 +1026,7 @@ Proof. lift_decide_eq. Defined.
 
 Instance eq_dec_SS_state : eq_dec SS.state.
 Proof. lift_decide_eq. Defined.
-*)
+
 (*
 The following are not true. 
 Instance eq_dec_effects `{eq_dec D} : eq_dec (effects D).
